Solve Smallstep.v!

plf/Smallstep.v
@@ -203,7 +203,10 @@ Example test_step_2 :
           (C 2)
           (C 4)).
 Proof.
-  (* FILL IN HERE *) Admitted.
+  constructor.
+  constructor.
+  constructor.
+Qed.
 (** [] *)
 
 End SimpleArith1.
@@ -464,7 +467,18 @@ Inductive step : tm -> tm -> Prop :=
 Theorem step_deterministic :
   deterministic step.
 Proof.
-  (* FILL IN HERE *) Admitted.
+  unfold deterministic.
+  intros x y1 y2 Hy1 Hy2.
+  generalize dependent y2.
+  induction Hy1; intros y2 Hy2.
+  - inversion Hy2; subst; try solve_by_invert. reflexivity.
+  - inversion Hy2; subst.
+    + solve_by_invert.
+    + apply IHHy1 in H2. rewrite H2. reflexivity.
+    + destruct H1. solve_by_invert.
+  - destruct H. inversion Hy2; subst; try solve_by_invert.
+    apply IHHy1 in H3. rewrite H3. reflexivity.
+Qed.
 (** [] *)
 
 (* ================================================================= *)
@@ -617,7 +631,12 @@ Inductive step : tm -> tm -> Prop :=
 Lemma value_not_same_as_normal_form :
   exists v, value v /\ ~ normal_form step v.
 Proof.
-  (* FILL IN HERE *) Admitted.
+  exists (P (C 1) (C 1)).
+  split.
+  - constructor.
+  - intros H. apply H. clear H.
+    exists (C 2). constructor.
+Qed.
 End Temp1.
 
 (** [] *)
@@ -652,7 +671,12 @@ Inductive step : tm -> tm -> Prop :=
 Lemma value_not_same_as_normal_form :
   exists v, value v /\ ~ normal_form step v.
 Proof.
-  (* FILL IN HERE *) Admitted.
+  exists (C 1).
+  split.
+  - constructor.
+  - intros H. apply H. clear H.
+    exists (P (C 1) (C 0)). constructor.
+Qed.
 
 End Temp2.
 (** [] *)
@@ -687,7 +711,13 @@ Inductive step : tm -> tm -> Prop :=
 Lemma value_not_same_as_normal_form :
   exists t, ~ value t /\ normal_form step t.
 Proof.
-  (* FILL IN HERE *) Admitted.
+  exists (P (C 0) (P (C 0) (C 1))).
+  split.
+  - intros contra. inversion contra.
+  - intros contra. destruct contra.
+    inversion H; subst.
+    inversion H3; subst.
+Qed.
 
 End Temp3.
 (** [] *)
@@ -732,7 +762,8 @@ Inductive step : tm -> tm -> Prop :=
 Definition bool_step_prop1 :=
   fls --> fls.
 
-(* FILL IN HERE *)
+Example bool_step_prop1_false : ~ bool_step_prop1.
+Proof. intros contra. inversion contra. Qed.
 
 Definition bool_step_prop2 :=
      test
@@ -742,7 +773,8 @@ Definition bool_step_prop2 :=
   -->
      tru.
 
-(* FILL IN HERE *)
+Example bool_step_prop2_false : ~ bool_step_prop2.
+Proof. intros contra. inversion contra. Qed.
 
 Definition bool_step_prop3 :=
      test
@@ -755,7 +787,8 @@ Definition bool_step_prop3 :=
        (test tru tru tru)
        fls.
 
-(* FILL IN HERE *)
+Example bool_step_prop3_false : bool_step_prop3.
+Proof. constructor. constructor. Qed.
 
 (* Do not modify the following line: *)
 Definition manual_grade_for_smallstep_bools : option (nat*string) := None.
@@ -769,13 +802,30 @@ Definition manual_grade_for_smallstep_bools : option (nat*string) := None.
 Theorem strong_progress_bool : forall t,
   value t \/ (exists t', t --> t').
 Proof.
-  (* FILL IN HERE *) Admitted.
+  intros.
+  induction t.
+  - left. constructor.
+  - left. constructor.
+  - right. destruct IHt1.
+    + inversion H; subst.
+      * exists t2. constructor.
+      * exists t3. constructor.
+    + destruct H as [t' H].
+      exists (test t' t2 t3). constructor. apply H.
+Qed.
 (** [] *)
 
 (** **** Exercise: 2 stars, standard, optional (step_deterministic) *)
 Theorem step_deterministic : deterministic step.
 Proof.
-  (* FILL IN HERE *) Admitted.
+  unfold deterministic.
+  intros x y1 y2 Hy1 Hy2.
+  generalize dependent y2.
+  induction Hy1; intros y2 Hy2; inversion Hy2; subst; try solve_by_invert.
+  - reflexivity.
+  - reflexivity.
+  - apply IHHy1 in H3. rewrite H3. reflexivity.
+Qed.
 (** [] *)
 
 Module Temp5.
@@ -811,7 +861,9 @@ Inductive step : tm -> tm -> Prop :=
   | ST_If : forall t1 t1' t2 t3,
       t1 --> t1' ->
       test t1 t2 t3 --> test t1' t2 t3
-  (* FILL IN HERE *)
+  | ST_ShortCircuit : forall t t',
+      value t' ->
+      test t t' t' --> t'
 
   where " t '-->' t' " := (step t t').
 
@@ -826,7 +878,7 @@ Definition bool_step_prop4 :=
 Example bool_step_prop4_holds :
   bool_step_prop4.
 Proof.
-  (* FILL IN HERE *) Admitted.
+  constructor. constructor. Qed.
 (** [] *)
 
 (** **** Exercise: 3 stars, standard, optional (properties_of_altered_step)
@@ -842,12 +894,20 @@ Proof.
 
       Optional: prove your answer correct in Coq. *)
 
-(* FILL IN HERE
-   - Does a strong progress theorem hold? Write yes or no and
-     briefly (1 sentence) explain your answer.
-
-     Optional: prove your answer correct in Coq.
-*)
+Theorem step_non_deterministic:
+  ~ deterministic step.
+Proof.
+  unfold deterministic.
+  intros contra.
+  assert (test tru tru tru = tru).
+  {
+    rewrite (contra (test (test tru tru tru) tru tru) (test tru tru tru) tru).
+    - reflexivity.
+    - constructor. constructor.
+    - constructor. constructor.
+  }
+  discriminate.
+Qed.
 
 (* FILL IN HERE
    - In general, is there any way we could cause strong progress to
@@ -1011,7 +1071,7 @@ Qed.
 Lemma test_multistep_2:
   C 3 -->* C 3.
 Proof.
-  (* FILL IN HERE *) Admitted.
+  constructor. Qed.
 (** [] *)
 
 (** **** Exercise: 1 star, standard, optional (test_multistep_3) *)
@@ -1020,7 +1080,7 @@ Lemma test_multistep_3:
    -->*
       P (C 0) (C 3).
 Proof.
-  (* FILL IN HERE *) Admitted.
+  constructor. Qed.
 (** [] *)
 
 (** **** Exercise: 2 stars, standard (test_multistep_4) *)
@@ -1035,7 +1095,18 @@ Lemma test_multistep_4:
         (C 0)
         (C (2 + (0 + 3))).
 Proof.
-  (* FILL IN HERE *) Admitted.
+  econstructor.
+  - apply ST_Plus2.
+    * constructor.
+    * apply ST_Plus2.
+      ** constructor.
+      ** constructor.
+  - econstructor.
+    * apply ST_Plus2.
+      ** constructor.
+      ** constructor.
+    * constructor.
+Qed.
 (** [] *)
 
 (* ================================================================= *)
@@ -1066,7 +1137,18 @@ Proof.
   intros x y1 y2 P1 P2.
   destruct P1 as [P11 P12].
   destruct P2 as [P21 P22].
-  (* FILL IN HERE *) Admitted.
+  induction P11.
+  - inversion P21; subst.
+    + reflexivity.
+    + exfalso. apply P12. exists y. assumption.
+  - apply IHP11.
+    + assumption.
+    + inversion P21; subst.
+      * exfalso. apply P22. exists y. assumption.
+      * replace y with y0.
+        ** assumption.
+        ** apply (step_deterministic x y0 y); assumption.
+Qed.
 (** [] *)
 
 (** Indeed, something stronger is true for this language (though
@@ -1103,7 +1185,14 @@ Lemma multistep_congr_2 : forall v1 t2 t2',
      t2 -->* t2' ->
      P v1 t2 -->* P v1 t2'.
 Proof.
-  (* FILL IN HERE *) Admitted.
+  intros v1 t2 t2' Hvalue H. induction H.
+  - apply multi_refl.
+  - apply multi_step with (P v1 y).
+    + apply ST_Plus2.
+      * apply Hvalue.
+      * apply H.
+    + apply IHmulti.
+Qed.
 (** [] *)
 
 (** With these lemmas in hand, the main proof is a straightforward
@@ -1215,7 +1304,19 @@ Theorem eval__multistep : forall t n,
     includes [-->]. *)
 
 Proof.
-  (* FILL IN HERE *) Admitted.
+  intros t n H.
+  induction H.
+  - apply multi_refl.
+  - eapply multi_trans.
+    + apply multistep_congr_1. apply IHeval1.
+    + eapply multi_trans.
+      * apply multistep_congr_2.
+        ** constructor.
+        ** apply IHeval2.
+      * eapply multi_step.
+        ** constructor.
+        ** apply multi_refl.
+Qed.
 (** [] *)
 
 (** **** Exercise: 3 stars, advanced (eval__multistep_inf)
@@ -1239,7 +1340,15 @@ Lemma step__eval : forall t t' n,
      t  ==> n.
 Proof.
   intros t t' n Hs. generalize dependent n.
-  (* FILL IN HERE *) Admitted.
+  induction Hs; intros.
+  - inversion H; subst. constructor; constructor.
+  - inversion H; subst. constructor.
+    + apply IHHs. assumption.
+    + assumption.
+  - destruct H. inversion H0; subst. constructor.
+    + assumption.
+    + apply IHHs. assumption.
+Qed.
 (** [] *)
 
 (** The fact that small-step reduction implies big-step evaluation is now
@@ -1255,7 +1364,21 @@ Proof.
 Theorem multistep__eval : forall t t',
   normal_form_of t t' -> exists n, t' = C n /\ t ==> n.
 Proof.
-  (* FILL IN HERE *) Admitted.
+  intros t t' H.
+  destruct H as [H Hnf].
+  unfold step_normal_form in Hnf. unfold normal_form in Hnf.
+  induction H as [t | t1 t2 t3 H12 H23].
+  - destruct (strong_progress t).
+    + destruct H as [n']. exists n'. split.
+      * reflexivity.
+      * constructor.
+    + exfalso. apply Hnf. apply H.
+  - destruct (IHH23 Hnf) as [n' [H H2]].
+    subst. exists n'.
+    split.
+    + reflexivity.
+    + apply step__eval with (t' := t2); assumption.
+Qed.
 (** [] *)
 
 (* ================================================================= *)
@@ -1272,7 +1395,14 @@ Proof.
 Theorem evalF_eval : forall t n,
   evalF t = n <-> t ==> n.
 Proof.
-  (* FILL IN HERE *) Admitted.
+  intros. split.
+  - intros. subst. induction t.
+    + constructor.
+    + simpl. constructor; assumption.
+  - intros. induction H.
+    + reflexivity.
+    + simpl. subst. reflexivity.
+Qed.
 (** [] *)
 
 (** We've considered arithmetic and conditional expressions
@@ -1326,7 +1456,25 @@ Inductive step : tm -> tm -> Prop :=
 (** **** Exercise: 3 stars, standard (combined_step_deterministic) *)
 Theorem combined_step_deterministic: (deterministic step) \/ ~ (deterministic step).
 Proof.
-  (* FILL IN HERE *) Admitted.
+  left.
+  unfold deterministic.
+  intros x y1 y2 Hy1 Hy2.
+  generalize dependent y2.
+  induction Hy1; intros y2 Hy2.
+  - inversion Hy2; subst; try solve_by_invert; reflexivity.
+  - inversion Hy2; subst.
+    + solve_by_invert.
+    + apply IHHy1 in H2. rewrite H2. reflexivity.
+    + destruct H1; solve_by_invert.
+  - destruct H; inversion Hy2; subst; try solve_by_invert;
+    apply IHHy1 in H3; rewrite H3; reflexivity.
+  - inversion Hy2; subst; try solve_by_invert; reflexivity.
+  - inversion Hy2; subst; try solve_by_invert; reflexivity.
+  - inversion Hy2; subst.
+    + inversion Hy1.
+    + inversion Hy1.
+    + apply IHHy1 in H3. rewrite H3. reflexivity.
+Qed.
 
 (** [] *)
 
@@ -1335,7 +1483,12 @@ Theorem combined_strong_progress :
   (forall t, value t \/ (exists t', t --> t'))
   \/ ~ (forall t, value t \/ (exists t', t --> t')).
 Proof.
-  (* FILL IN HERE *) Admitted.
+  right.
+  intros H.
+  destruct (H (P (C 1) tru)) as [contra | [t contra]].
+  - inversion contra.
+  - inversion contra; subst; solve_by_invert.
+Qed.
 (** [] *)
 
 End Combined.
@@ -1707,7 +1860,25 @@ Lemma par_body_n__Sn : forall n st,
   st X = n /\ st Y = 0 ->
   par_loop / st -->* par_loop / (X !-> S n ; st).
 Proof.
-  (* FILL IN HERE *) Admitted.
+  intros n st [HX HY].
+  eapply multi_step.
+  - apply CS_Par2. constructor.
+  - eapply multi_step.
+    + apply CS_Par2. apply CS_IfStep. apply BS_Eq1. apply AS_Id.
+    + eapply multi_step.
+      * apply CS_Par2. apply CS_IfStep. apply BS_Eq.
+      * rewrite HY. simpl. eapply multi_step.
+        -- apply CS_Par2. apply CS_IfTrue.
+        -- eapply multi_step.
+           ++ apply CS_Par2. apply CS_SeqStep. apply CS_AsgnStep. apply AS_Plus1. apply AS_Id.
+           ++ eapply multi_step.
+              ** rewrite HX. apply CS_Par2. apply CS_SeqStep. apply CS_AsgnStep. apply AS_Plus.
+              ** eapply multi_step.
+                 --- apply CS_Par2. apply CS_SeqStep. apply CS_Asgn.
+                 --- eapply multi_step.
+                     +++ apply CS_Par2. apply CS_SeqFinish.
+                     +++ rewrite Nat.add_comm. apply multi_refl.
+Qed.
 (** [] *)
 
 (** **** Exercise: 3 stars, standard, optional (par_body_n) *)
@@ -1716,7 +1887,35 @@ Lemma par_body_n : forall n st,
   exists st',
     par_loop / st -->*  par_loop / st' /\ st' X = n /\ st' Y = 0.
 Proof.
-  (* FILL IN HERE *) Admitted.
+  intros n st [HX HY].
+  induction n as [| n [st' [IH [HX' HY']]]].
+  - exists st. split.
+    + apply multi_refl.
+    + split; assumption.
+  - exists (X !-> S n ; st'). split.
+    + eapply multi_trans.
+      * apply IH.
+      * eapply multi_step.
+        -- apply CS_Par2. apply CS_While.
+        -- eapply multi_step.
+           ++ apply CS_Par2. apply CS_IfStep. apply BS_Eq1. apply AS_Id.
+           ++ eapply multi_step.
+              ** apply CS_Par2. rewrite HY'. apply CS_IfStep. apply BS_Eq.
+              ** eapply multi_step.
+                 --- apply CS_Par2. apply CS_IfTrue.
+                 --- eapply multi_step.
+                     +++ apply CS_Par2. apply CS_SeqStep. apply CS_AsgnStep. apply AS_Plus1. apply AS_Id.
+                     +++ eapply multi_step.
+                         *** apply CS_Par2. rewrite HX'. apply CS_SeqStep. apply CS_AsgnStep. apply AS_Plus.
+                         *** eapply multi_step.
+                             ---- apply CS_Par2. apply CS_SeqStep. apply CS_Asgn.
+                             ---- eapply multi_step.
+                                  ++++ apply CS_Par2. apply CS_SeqFinish.
+                                  ++++ rewrite Nat.add_comm. apply multi_refl.
+    + split.
+      * reflexivity.
+      * rewrite <- HY'. apply t_update_neq. apply eqb_neq. reflexivity.
+Qed.
 (** [] *)
 
 (** ... the above loop can exit with [X] having any value
@@ -1798,14 +1997,60 @@ Definition stack_multistep st := multi (stack_step st).
     what it means for the compiler to be correct according to the
     stack machine small step semantics, and then prove it. *)
 
-(* Copy your definition of s_compile here *)
+Fixpoint s_compile (e : aexp) : list sinstr
+  := match e with
+     | ANum n => [SPush n]
+     | AId x => [SLoad x]
+     | APlus a1 a2 => s_compile a1 ++ s_compile a2 ++ [SPlus]
+     | AMinus a1 a2 => s_compile a1 ++ s_compile a2 ++ [SMinus]
+     | AMult a1 a2 => s_compile a1 ++ s_compile a2 ++ [SMult]
+     end.
 
 Definition compiler_is_correct_statement : Prop
-  (* REPLACE THIS LINE WITH ":= _your_definition_ ." *). Admitted.
+  := forall (st : state) (e : aexp),
+     stack_multistep st (s_compile e, nil) (nil, [ aeval st e ]).
+
+Lemma compiler_is_correct_aux:
+  forall (st : state) (e : aexp) (stk : stack) (p : prog),
+    stack_multistep st (s_compile e ++ p, stk) (p, aeval st e :: stk).
+Proof.
+  unfold compiler_is_correct_statement.
+  intros st e. generalize dependent st. induction e; intros st stk p.
+  - eapply multi_step.
+    + apply SS_Push.
+    + apply multi_refl.
+  - eapply multi_step.
+    + apply SS_Load.
+    + apply multi_refl.
+  - eapply multi_trans.
+    + simpl. rewrite <- app_assoc. apply IHe1.
+    + eapply multi_trans.
+      * rewrite <- app_assoc. apply IHe2.
+      * eapply multi_step.
+        -- apply SS_Plus.
+        -- simpl. apply multi_refl.
+  - eapply multi_trans.
+    + simpl. rewrite <- app_assoc. apply IHe1.
+    + eapply multi_trans.
+      * rewrite <- app_assoc. apply IHe2.
+      * eapply multi_step.
+        -- apply SS_Minus.
+        -- simpl. apply multi_refl.
+  - eapply multi_trans.
+    + simpl. rewrite <- app_assoc. apply IHe1.
+    + eapply multi_trans.
+      * rewrite <- app_assoc. apply IHe2.
+      * eapply multi_step.
+        -- apply SS_Mult.
+        -- simpl. apply multi_refl.
+Qed.
 
 Theorem compiler_is_correct : compiler_is_correct_statement.
 Proof.
-(* FILL IN HERE *) Admitted.
+  unfold compiler_is_correct_statement. intros.
+  rewrite <- app_nil_r with (l := s_compile e).
+  apply compiler_is_correct_aux.
+Qed.
 (** [] *)
 
 (* ################################################################# *)
@@ -1895,7 +2140,10 @@ Theorem normalize_ex : exists e',
   (P (C 3) (P (C 2) (C 1)))
   -->* e' /\ value e'.
 Proof.
-  (* FILL IN HERE *) Admitted.
+  eexists. split.
+  - normalize.
+  - auto.
+Qed.
 (** [] *)
 
 (** **** Exercise: 1 star, standard, optional (normalize_ex')
@@ -1906,7 +2154,16 @@ Theorem normalize_ex' : exists e',
   (P (C 3) (P (C 2) (C 1)))
   -->* e' /\ value e'.
 Proof.
-  (* FILL IN HERE *) Admitted.
+  exists (C 6). split.
+  - apply multi_step with (P (C 3) (C 3)).
+    + apply ST_Plus2.
+      * apply v_const.
+      * apply ST_PlusConstConst.
+    + apply multi_step with (C 6).
+      * apply ST_PlusConstConst.
+      * apply multi_refl.
+  - apply v_const.
+Qed.
 (** [] *)
 
 (* 2025-08-24 13:47 *)
